tll session

coq_session/dyn_type.v
@@ -8,36 +8,142 @@ Set Implicit Arguments.
 Unset Strict Implicit.
 Unset Printing Implicit Defensive.
 
-Reserved Notation "Γ ; Δ ⊢ m : A" (at level 50, Δ, m, A at next level).
-Inductive dyn_type : sta_ctx -> dyn_ctx -> term -> term -> Prop :=
-| dyn_var Γ Δ x s A :
+Reserved Notation "Γ ; Δ ; Θ ⊢ m : A"
+  (at level 50, Δ, Θ, m, A at next level).
+Inductive dyn_type : sta_ctx -> dyn_ctx -> dyn_ctx -> term -> term -> Prop :=
+(* core *)
+| dyn_var Γ Δ Θ x s A :
   dyn_wf Γ Δ ->
   sta_has Γ x A ->
   dyn_has Δ x s A ->
-  Γ ; Δ ⊢ Var x : A
-| dyn_lam0 Γ Δ A B m s :
+  dyn_empty Θ ->
+  Γ ; Δ ; Θ ⊢ Var x : A
+| dyn_lam0 Γ Δ Θ A B m s :
   Δ ▷ s ->
-  (A :: Γ) ; _: Δ ⊢ m : B ->
-  Γ ; Δ ⊢ Lam0 A m s : Pi0 A B s
-| dyn_lam1 Γ Δ A B m s t :
+  Θ ▷ s ->
+  (A :: Γ) ; _: Δ ; Θ ⊢ m : B ->
+  Γ ; Δ ; Θ ⊢ Lam0 A m s : Pi0 A B s
+| dyn_lam1 Γ Δ Θ A B m s t :
   Δ ▷ s ->
-  (A :: Γ) ; A :{t} Δ ⊢ m : B ->
-  Γ ; Δ ⊢ Lam1 A m s : Pi1 A B s
-| dyn_app0 Γ Δ A B m n s :
-  Γ ; Δ ⊢ m : Pi0 A B s ->
+  Θ ▷ s ->
+  (A :: Γ) ; A :{t} Δ ; Θ ⊢ m : B ->
+  Γ ; Δ ; Θ ⊢ Lam1 A m s : Pi1 A B s
+| dyn_app0 Γ Δ Θ A B m n s :
+  Γ ; Δ ; Θ ⊢ m : Pi0 A B s ->
   Γ ⊢ n : A ->
-  Γ ; Δ ⊢ App m n : B.[n/]
-| dyn_app1 Γ Δ1 Δ2 Δ A B m n s :
+  Γ ; Δ ; Θ ⊢ App m n : B.[n/]
+| dyn_app1 Γ Δ1 Δ2 Δ Θ1 Θ2 Θ A B m n s :
   Δ1 ∘ Δ2 => Δ ->
-  Γ ; Δ1 ⊢ m : Pi1 A B s ->
-  Γ ; Δ2 ⊢ n : A ->
-  Γ ; Δ ⊢ App m n : B.[n/]
-| dyn_conv Γ Δ A B m s :
+  Θ1 ∘ Θ2 => Θ ->
+  Γ ; Δ1 ; Θ1 ⊢ m : Pi1 A B s ->
+  Γ ; Δ2 ; Θ2 ⊢ n : A ->
+  Γ ; Δ ; Θ ⊢ App m n : B.[n/]
+| dyn_pair0 Γ Δ Θ A B m n t :
+  Γ ⊢ Sig0 A B t : Sort t ->
+  Γ ; Δ ; Θ ⊢ m : A ->
+  Γ ⊢ n : B.[m/] ->
+  Γ ; Δ ; Θ ⊢ Pair0 m n t : Sig0 A B t
+| dyn_pair1 Γ Δ1 Δ2 Δ Θ1 Θ2 Θ A B m n t :
+  Δ1 ∘ Δ2 => Δ ->
+  Θ1 ∘ Θ2 => Θ ->
+  Γ ⊢ Sig1 A B t : Sort t ->
+  Γ ; Δ1 ; Θ1 ⊢ m : A ->
+  Γ ; Δ2 ; Θ2 ⊢ n : B.[m/] ->
+  Γ ; Δ ; Θ ⊢ Pair1 m n t : Sig1 A B t
+| dyn_letin0 Γ Δ1 Δ2 Δ Θ1 Θ2 Θ A B C m n s r t :
+  Δ1 ∘ Δ2 => Δ ->
+  Θ1 ∘ Θ2 => Θ ->
+  (Sig0 A B t :: Γ) ⊢ C : Sort s ->
+  Γ ; Δ1 ; Θ1 ⊢ m : Sig0 A B t ->
+  (B :: A :: Γ) ; _: A :{r} Δ2 ; Θ2 ⊢ n : C.[Pair0 (Var 1) (Var 0) t .: ren (+2)] ->
+  Γ ; Δ ; Θ ⊢ LetIn C m n : C.[m/]
+| dyn_letin1 Γ Δ1 Δ2 Δ Θ1 Θ2 Θ A B C m n s r1 r2 t :
+  Δ1 ∘ Δ2 => Δ ->
+  Θ1 ∘ Θ2 => Θ ->
+  (Sig1 A B t :: Γ) ⊢ C : Sort s ->
+  Γ ; Δ1 ; Θ1 ⊢ m : Sig1 A B t ->
+  (B :: A :: Γ) ; B :{r2} A :{r1} Δ2 ; Θ2 ⊢ n : C.[Pair1 (Var 1) (Var 0) t .: ren (+2)] ->
+  Γ ; Δ ; Θ ⊢ LetIn C m n : C.[m/]
+| dyn_sta_fix Γ Δ Θ A m :
+  Δ ▷ U ->
+  Θ ▷ U ->
+  (A :: Γ) ; A :U Δ ; Θ ⊢ m : A.[ren (+1)] ->
+  Γ ; Δ ; Θ ⊢ Fix A m : A
+(* data *)
+| dyn_ii Γ Δ Θ :
+  Δ ▷ U ->
+  dyn_wf Γ Δ ->
+  dyn_empty Θ ->
+  Γ ; Δ ; Θ ⊢ II : Unit
+| dyn_tt Γ Δ Θ :
+  Δ ▷ U ->
+  dyn_wf Γ Δ ->
+  dyn_empty Θ ->
+  Γ ; Δ ; Θ ⊢ TT : Bool
+| dyn_ff Γ Δ Θ :
+  Δ ▷ U ->
+  dyn_wf Γ Δ ->
+  dyn_empty Θ ->
+  Γ ; Δ ; Θ ⊢ FF : Bool
+| dyn_ifte Γ Δ1 Δ2 Δ Θ1 Θ2 Θ A m n1 n2 s :
+  Δ1 ∘ Δ2 => Δ ->
+  Θ1 ∘ Θ2 => Θ ->
+  Γ ; Δ1 ; Θ1 ⊢ m : Bool ->
+  (Bool :: Γ) ⊢ A : Sort s ->
+  Γ ; Δ2 ; Θ2 ⊢ n1 : A.[TT/] ->
+  Γ ; Δ2 ; Θ2 ⊢ n2 : A.[FF/] ->
+  Γ ; Δ ; Θ ⊢ Ifte A m n1 n2 : A.[m/]
+(* monadic *)
+| dyn_return Γ Δ Θ m A :
+  Γ ; Δ ; Θ ⊢ m : A ->
+  Γ ; Δ ; Θ ⊢ Return m : IO A
+| dyn_bind Γ Δ1 Δ2 Δ Θ1 Θ2 Θ m n A B s t :
+  Δ1 ∘ Δ2 => Δ ->
+  Θ1 ∘ Θ2 => Θ ->
+  Γ ⊢ B : Sort t ->
+  Γ ; Δ1 ; Θ1 ⊢ m : IO A ->
+  (A :: Γ) ; (A :{s} Δ2) ; Θ2 ⊢ n : IO B.[ren (+1)] ->
+  Γ ; Δ ; Θ ⊢ Bind m n : IO B
+(* session *)
+| dyn_cvar Γ Δ Θ r x A :
+  Δ ▷ U ->
+  Γ ⊢ A : Proto ->
+  dyn_just Θ x (Ch r A) ->
+  Γ ; Δ ; Θ ⊢ CVar x : Ch r A
+| dyn_fork Γ Δ Θ m A :
+  (Ch true A :: Γ) ; Ch true A :L Δ ; Θ ⊢ m : IO Unit ->
+  Γ ; Δ ; Θ ⊢ Fork A m : IO (Ch false A)
+| dyn_recv0 Γ Δ Θ r1 r2 A B m :
+  r1 (+) r2 = false ->
+  Γ ; Δ ; Θ ⊢ m : Ch r1 (Act0 r2 A B) ->
+  Γ ; Δ ; Θ ⊢ Recv m : IO (Sig0 A (Ch r1 B) L)
+| dyn_recv1 Γ Δ Θ r1 r2 A B m :
+  r1 (+) r2 = false ->
+  Γ ; Δ ; Θ ⊢ m : Ch r1 (Act1 r2 A B) ->
+  Γ ; Δ ; Θ ⊢ Recv m : IO (Sig1 A (Ch r1 B) L)
+| dyn_send0 Γ Δ Θ r1 r2 A B m :
+  r1 (+) r2 = true ->
+  Γ ; Δ ; Θ ⊢ m : Ch r1 (Act0 r2 A B) ->
+  Γ ; Δ ; Θ ⊢ Send m : Pi0 A (IO (Ch r1 B)) L
+| dyn_send1 Γ Δ Θ r1 r2 A B m :
+  r1 (+) r2 = true ->
+  Γ ; Δ ; Θ ⊢ m : Ch r1 (Act1 r2 A B) ->
+  Γ ; Δ ; Θ ⊢ Send m : Pi1 A (IO (Ch r1 B)) L
+| dyn_wait Γ Δ Θ r1 r2 m :
+  r1 (+) r2 = false ->
+  Γ ; Δ ; Θ ⊢ m : Ch r1 (Stop r2) ->
+  Γ ; Δ ; Θ ⊢ Wait m : IO Unit
+| dyn_close Γ Δ Θ r1 r2 m :
+  r1 (+) r2 = true ->
+  Γ ; Δ ; Θ ⊢ m : Ch r1 (Stop r2) ->
+  Γ ; Δ ; Θ ⊢ Close m : IO Unit
+(* conversion *)
+| dyn_conv Γ Δ Θ A B m s :
   A === B ->
-  Γ ; Δ ⊢ m : A ->
+  Γ ; Δ ; Θ ⊢ m : A ->
   Γ ⊢ B : Sort s ->
-  Γ ; Δ ⊢ m : B
-where "Γ ; Δ ⊢ m : A" := (dyn_type Γ Δ m A)
+  Γ ; Δ ; Θ ⊢ m : B
+where "Γ ; Δ ; Θ ⊢ m : A" := (dyn_type Γ Δ Θ m A)
 
 with dyn_wf : sta_ctx -> dyn_ctx -> Prop :=
 | dyn_wf_nil : dyn_wf nil nil
@@ -66,12 +172,12 @@ Proof with eauto using dyn_wf.
     { inv wf2. apply: dyn_wf_n... } }
 Qed.
 
-Lemma dyn_type_wf Γ Δ m A : Γ ; Δ ⊢ m : A -> dyn_wf Γ Δ.
-Proof with eauto using dyn_wf.
-  elim=>{Γ Δ m A}...
-  { move=>Γ Δ A B m s k tym ih. inv ih... }
-  { move=>Γ Δ A B m s t k tym ih. inv ih... }
-  { move=>Γ Δ1 Δ2 Δ A B m n s mrg tym ihm tyn ihn.
+Lemma dyn_type_wf Γ Δ Θ m A : Γ ; Δ ; Θ ⊢ m : A -> dyn_wf Γ Δ.
+Proof with eauto 8 using dyn_wf.
+  elim=>{Γ Δ Θ m A}...
+  { move=>Γ Δ Θ A B m s k1 k2 tym ih. inv ih... }
+  { move=>Γ Δ Θ A B m s t k1 k2 tym ih. inv ih... }
+  { move=>Γ Δ1 Δ2 Δ Θ1 Θ2 Θ A B m n s mrg tym ihm tyn ihn.
     apply: dyn_wf_merge... }
 Qed.
 Hint Resolve dyn_type_wf.
