coq_session/dyn_step.v
@@ -8,23 +8,93 @@ Unset Printing Implicit Defensive.
 
 Inductive dyn_val : term -> Prop :=
 | dyn_val_var x : dyn_val (Var x)
-| dyn_val_lam0 A B s : dyn_val (Lam0 A B s)
-| dyn_val_lam1 A B s : dyn_val (Lam1 A B s).
+| dyn_val_lam0 A m s : dyn_val (Lam0 A m s)
+| dyn_val_lam1 A m s : dyn_val (Lam1 A m s)
+| dyn_val_pair0 m1 m2 s :
+  dyn_val m1 ->
+  dyn_val (Pair0 m1 m2 s)
+| dyn_val_pair1 m1 m2 s :
+  dyn_val m1 ->
+  dyn_val m2 ->
+  dyn_val (Pair1 m1 m2 s)
+| dyn_val_ii : dyn_val II
+| dyn_val_tt : dyn_val TT
+| dyn_val_ff : dyn_val FF
+| dyn_val_return v : dyn_val v -> dyn_val (Return v)
+| dyn_val_bind v n : dyn_val v -> dyn_val (Bind v n)
+| dyn_val_cvar x : dyn_val (CVar x)
+| dyn_val_fork A v : dyn_val v -> dyn_val (Fork A v)
+| dyn_val_recv v : dyn_val v -> dyn_val (Recv v)
+| dyn_val_send v : dyn_val v -> dyn_val (Send v)
+| dyn_val_close v : dyn_val v -> dyn_val (Close v)
+| dyn_val_wait v : dyn_val v -> dyn_val (Wait v).
 
-Reserved Notation "m ~>> n" (at level 30).
+Reserved Notation "m ~>> n" (at level 50).
 Inductive dyn_step : term -> term -> Prop :=
-| dyn_appL m m' n :
+(* core *)
+| dyn_step_appL m m' n :
   m ~>> m' ->
   App m n ~>> App m' n
-| dyn_appR m n n' :
+| dyn_step_appR m n n' :
   n ~>> n' ->
   App m n ~>> App m n'
-| dyn_beta0 A m n s :
+| dyn_step_beta0 A m n s :
   App (Lam0 A m s) n ~>> m.[n/]
-| dyn_beta1 A m v s :
+| dyn_step_beta1 A m v s :
   dyn_val v ->
   App (Lam1 A m s) v ~>> m.[v/]
+| dyn_step_pair0L m m' n s :
+  m ~>> m' ->
+  Pair0 m n s ~>> Pair0 m' n s
+| dyn_step_pair1L m m' n s :
+  m ~>> m' ->
+  Pair1 m n s ~>> Pair1 m' n s
+| dyn_step_pair1R m n n' s :
+  n ~>> n' ->
+  Pair1 m n s ~>> Pair1 m n' s
+| dyn_step_letinL A m m' n :
+  m ~>> m' ->
+  LetIn A m n ~>> LetIn A m' n
+| dyn_step_letinE0 A m1 m2 n s :
+  dyn_val (Pair0 m1 m2 s) ->
+  LetIn A (Pair0 m1 m2 s) n ~>> n.[m2,m1/]
+| dyn_step_letinE1 A m1 m2 n s :
+  dyn_val (Pair1 m1 m2 s) ->
+  LetIn A (Pair1 m1 m2 s) n ~>> n.[m2,m1/]
+| dyn_step_fixE A m :
+  Fix A m ~>> m.[Fix A m/]
+(* data *)
+| dyn_step_ifteM A m m' n1 n2 :
+  m ~>> m' ->
+  Ifte A m n1 n2 ~>> Ifte A m' n1 n2
+| dyn_step_ifteT A n1 n2 :
+  Ifte A TT n1 n2 ~>> n1
+| dyn_step_ifteF A n1 n2 :
+  Ifte A FF n1 n2 ~>> n2
+(* monadic *)
+| dyn_step_return m m' :
+  m ~>> m' ->
+  Return m ~>> Return m'
+| dyn_step_bindL m m' n :
+  m ~>> m' ->
+  Bind m n ~>> Bind m' n
+(* session *)
+| dyn_step_forkR A m m' :
+  m ~>> m' ->
+  Fork A m ~>> Fork A m'
+| dyn_step_recv m m' :
+  m ~>> m' ->
+  Recv m ~>> Recv m'
+| dyn_step_send m m' :
+  m ~>> m' ->
+  Send m ~>> Send m'
+| dyn_step_close m m' :
+  m ~>> m' ->
+  Close m ~>> Close m'
+| dyn_step_wait m m' :
+  m ~>> m' ->
+  Wait m ~>> Wait m'
 where "m ~>> n" := (dyn_step m n).
 
 Notation dyn_red := (star dyn_step).
-Notation "m ~>>* n" := (dyn_red m n) (at level 30).
+Notation "m ~>>* n" := (dyn_red m n) (at level 50).
