coq_session/tll_nf.v
@@ -1,0 +1,233 @@
+From mathcomp Require Import ssreflect ssrbool eqtype ssrnat seq.
+From Coq Require Import ssrfun Classical Utf8.
+Require Export AutosubstSsr ARS tll_ast.
+
+Set Implicit Arguments.
+Unset Strict Implicit.
+Unset Printing Implicit Defensive.
+
+Inductive nf : nat -> term -> Prop :=
+(* core *)
+| nf_var i x :
+  x < i ->
+  nf i (Var x)
+| nf_sort i s :
+  nf i (Sort s)
+| nf_pi0 i A B s :
+  nf i A ->
+  nf i.+1 B ->
+  nf i (Pi0 A B s)
+| nf_pi1 i A B s :
+  nf i A ->
+  nf i.+1 B ->
+  nf i (Pi1 A B s)
+| nf_lam0 i A m s :
+  nf i A ->
+  nf i.+1 m ->
+  nf i (Lam0 A m s)
+| nf_lam1 i A m s :
+  nf i A ->
+  nf i.+1 m ->
+  nf i (Lam0 A m s)
+| nf_app i m n :
+  nf i m ->
+  nf i n ->
+  nf i (App m n)
+| nf_sig0 i A B s :
+  nf i A ->
+  nf i.+1 B ->
+  nf i (Sig0 A B s)
+| nf_sig1 i A B s :
+  nf i A ->
+  nf i.+1 B ->
+  nf i (Sig1 A B s)
+| nf_pair0 i m n s :
+  nf i m ->
+  nf i n ->
+  nf i (Pair0 m n s)
+| nf_pair1 i m n s :
+  nf i m ->
+  nf i n ->
+  nf i (Pair1 m n s)
+| nf_letin i A m n :
+  nf i.+1 A ->
+  nf i m ->
+  nf i.+2 n ->
+  nf i (LetIn A m n)
+| nf_fix i A m :
+  nf i A ->
+  nf i.+1 m ->
+  nf i (Fix A m)
+(* data *)
+| nf_unit i : nf i Unit
+| nf_ii i : nf i II
+| nf_bool i : nf i Bool
+| nf_tt i : nf i TT
+| nf_ff i : nf i FF
+| nf_ifte i A m n1 n2 :
+  nf i.+1 A ->
+  nf i m ->
+  nf i n1 ->
+  nf i n2 ->
+  nf i (Ifte A m n1 n2)
+(* monadic *)
+| nf_io i A :
+  nf i A ->
+  nf i (IO A)
+| nf_return i m :
+  nf i m ->
+  nf i (Return m)
+| nf_bind i m n :
+  nf i m ->
+  nf i.+1 n ->
+  nf i (Bind m n)
+(* session *)
+| nf_proto i : nf i Proto
+| nf_stop i r : nf i (Stop r)
+| nf_act0 i r A B :
+  nf i A ->
+  nf i.+1 B ->
+  nf i (Act0 r A B)
+| nf_act1 i r A B :
+  nf i A ->
+  nf i.+1 B ->
+  nf i (Act1 r A B)
+| nf_ch i r A :
+  nf i A ->
+  nf i (Ch r A)
+| nf_cvar i x : nf i (CVar x)
+| nf_fork i A m :
+  nf i A ->
+  nf i.+1 m ->
+  nf i (Fork A m)
+| nf_recv i m :
+  nf i m ->
+  nf i (Recv m)
+| nf_send i m :
+  nf i m ->
+  nf i (Send m)
+| nf_close i m :
+  nf i m ->
+  nf i (Close m)
+| nf_wait i m :
+  nf i m ->
+  nf i (Wait m).
+
+Definition id_ren i ξ := forall x, x < i -> ξ x = x.
+
+Lemma id_ren1 : id_ren 0 (+1).
+Proof. move=>x h. inv h. Qed.
+
+Lemma id_ren_up i ξ : id_ren i ξ -> id_ren i.+1 (upren ξ).
+Proof.
+  move=>idr x h.
+  destruct x.
+  asimpl. eauto.
+  asimpl. rewrite idr; eauto.
+Qed.
+
+Lemma nf_id_ren i m ξ : nf i m -> id_ren i ξ -> m = m.[ren ξ].
+Proof with eauto using id_ren_up.
+  move=>nfi. elim: nfi ξ=>{i m}...
+  { move=>i x lt ξ idr. asimpl. rewrite idr... }
+  { move=>i A B s nfA ihA nfB ihB ξ idr. asimpl.
+    rewrite<-ihA... rewrite<-ihB... }
+  { move=>i A B s nfA ihA nfB ihB ξ idr. asimpl.
+    rewrite<-ihA... rewrite<-ihB... }
+  { move=>i A m s nfA ihA nfm ihm ξ idr. asimpl.
+    rewrite<-ihA... rewrite<-ihm... }
+  { move=>i A m s nfA ihA nfm ihm ξ idr. asimpl.
+    rewrite<-ihA... rewrite<-ihm... }
+  { move=>i m n nfm ihm nfn ihn ξ idr. asimpl.
+    rewrite<-ihm... rewrite<-ihn... }
+  { move=>i A B s nfA ihA nfB ihB ξ idr. asimpl.
+    rewrite<-ihA... rewrite<-ihB... }
+  { move=>i A B s nfA ihA nfB ihB ξ idr. asimpl.
+    rewrite<-ihA... rewrite<-ihB... }
+  { move=>i m n s nfm ihm nfn ihn ξ idr. asimpl.
+    rewrite<-ihm... rewrite<-ihn... }
+  { move=>i m n s nfm ihm nfn ihn ξ idr. asimpl.
+    rewrite<-ihm... rewrite<-ihn... }
+  { move=>i A m n nfA ihA nfm ihm nfn ihn ξ idr. asimpl.
+    rewrite<-ihA... rewrite<-ihm...
+    have eq:=ihn _ (id_ren_up (id_ren_up idr)).
+    asimpl in eq. rewrite<-eq... }
+  { move=>i A m nfA ihA nfm ihm ξ idr. asimpl.
+    rewrite<-ihA... rewrite<-ihm... }
+  { move=>i A m n1 n2 nfA ihA nfm ihm nfn1 ihn1 nfn2 ihn2 ξ idr. asimpl.
+    rewrite<-ihA... rewrite<-ihm...
+    rewrite<-ihn1... rewrite<-ihn2... }
+  { move=>i A nfA ihA ξ idr. asimpl. rewrite<-ihA... }
+  { move=>i m nfm ihm ξ idr. asimpl. rewrite<-ihm... }
+  { move=>i m n nfm ihm nfn ihn ξ idr. asimpl.
+    rewrite<-ihm... rewrite<-ihn... }
+  { move=>i r A B nfA ihA nfB ihB ξ idr. asimpl.
+    rewrite<-ihA... rewrite<-ihB... }
+  { move=>i r A B nfA ihA nfB ihB ξ idr. asimpl.
+    rewrite<-ihA... rewrite<-ihB... }
+  { move=>i r A nfA ihA ξ idr. asimpl. rewrite<-ihA... }
+  { move=>i A m nfA ihA nfm ihm ξ idr. asimpl.
+    rewrite<-ihA... rewrite<-ihm... }
+  { move=>i m nfm ihm ξ idr. asimpl. rewrite<-ihm... }
+  { move=>i m nfm ihm ξ idr. asimpl. rewrite<-ihm... }
+  { move=>i m nfm ihm ξ idr. asimpl. rewrite<-ihm... }
+  { move=>i m nfm ihm ξ idr. asimpl. rewrite<-ihm... }
+Qed.
+
+Definition id_subst i σ := forall x, x < i -> σ x = Var x.
+
+Lemma id_subst_up i σ : id_subst i σ -> id_subst i.+1 (up σ).
+Proof.
+  move=>idr x h.
+  destruct x.
+  asimpl. eauto.
+  asimpl. rewrite idr; eauto.
+Qed.
+
+Lemma nf_id_subst i m σ : nf i m -> id_subst i σ -> m = m.[σ].
+Proof with eauto using id_subst_up.
+  move=>nfi. elim: nfi σ=>{i m}...
+  { move=>i x lt ξ idr. asimpl. rewrite idr... }
+  { move=>i A B s nfA ihA nfB ihB ξ idr. asimpl.
+    rewrite<-ihA... rewrite<-ihB... }
+  { move=>i A B s nfA ihA nfB ihB ξ idr. asimpl.
+    rewrite<-ihA... rewrite<-ihB... }
+  { move=>i A m s nfA ihA nfm ihm ξ idr. asimpl.
+    rewrite<-ihA... rewrite<-ihm... }
+  { move=>i A m s nfA ihA nfm ihm ξ idr. asimpl.
+    rewrite<-ihA... rewrite<-ihm... }
+  { move=>i m n nfm ihm nfn ihn ξ idr. asimpl.
+    rewrite<-ihm... rewrite<-ihn... }
+  { move=>i A B s nfA ihA nfB ihB ξ idr. asimpl.
+    rewrite<-ihA... rewrite<-ihB... }
+  { move=>i A B s nfA ihA nfB ihB ξ idr. asimpl.
+    rewrite<-ihA... rewrite<-ihB... }
+  { move=>i m n s nfm ihm nfn ihn ξ idr. asimpl.
+    rewrite<-ihm... rewrite<-ihn... }
+  { move=>i m n s nfm ihm nfn ihn ξ idr. asimpl.
+    rewrite<-ihm... rewrite<-ihn... }
+  { move=>i A m n nfA ihA nfm ihm nfn ihn ξ idr. asimpl.
+    rewrite<-ihA... rewrite<-ihm...
+    have eq:=ihn _ (id_subst_up (id_subst_up idr)).
+    asimpl in eq. rewrite<-eq... }
+  { move=>i A m nfA ihA nfm ihm ξ idr. asimpl.
+    rewrite<-ihA... rewrite<-ihm... }
+  { move=>i A m n1 n2 nfA ihA nfm ihm nfn1 ihn1 nfn2 ihn2 ξ idr. asimpl.
+    rewrite<-ihA... rewrite<-ihm...
+    rewrite<-ihn1... rewrite<-ihn2... }
+  { move=>i A nfA ihA ξ idr. asimpl. rewrite<-ihA... }
+  { move=>i m nfm ihm ξ idr. asimpl. rewrite<-ihm... }
+  { move=>i m n nfm ihm nfn ihn ξ idr. asimpl.
+    rewrite<-ihm... rewrite<-ihn... }
+  { move=>i r A B nfA ihA nfB ihB ξ idr. asimpl.
+    rewrite<-ihA... rewrite<-ihB... }
+  { move=>i r A B nfA ihA nfB ihB ξ idr. asimpl.
+    rewrite<-ihA... rewrite<-ihB... }
+  { move=>i r A nfA ihA ξ idr. asimpl. rewrite<-ihA... }
+  { move=>i A m nfA ihA nfm ihm ξ idr. asimpl.
+    rewrite<-ihA... rewrite<-ihm... }
+  { move=>i m nfm ihm ξ idr. asimpl. rewrite<-ihm... }
+  { move=>i m nfm ihm ξ idr. asimpl. rewrite<-ihm... }
+  { move=>i m nfm ihm ξ idr. asimpl. rewrite<-ihm... }
+  { move=>i m nfm ihm ξ idr. asimpl. rewrite<-ihm... }
+Qed.
